Able to do a few simple examples using the metaprogram

rupicola/io/Metaprogram.fst
@@ -2,6 +2,7 @@ module Metaprogram
 
 open HelperTactics
 
+open FStar.Tactics.Typeclasses
 open FStar.Tactics.V2
 open FStar.Reflection.Typing
 open FStar.Stubs.Reflection.V2.Builtins
@@ -16,18 +17,184 @@ let mk_tyj (ty t : term) : Tot term =
 let mk_qtt : term =
   mk_app (`Qtt) [(pack_ln Tv_Unknown, Q_Implicit)]
 
-let meta_translation (nm:string) (qprog:term) : dsl_tac_t = fun (g, expected_t) ->
+let mk_qtrue : term =
+  mk_app (`QTrue) [(pack_ln Tv_Unknown, Q_Implicit)]
+
+let mk_qfalse : term =
+  mk_app (`QFalse) [(pack_ln Tv_Unknown, Q_Implicit)]
+
+let mk_qvar0 : term =
+  mk_app (`QVar0) [
+    (pack_ln Tv_Unknown, Q_Implicit);
+    (pack_ln Tv_Unknown, Q_Implicit)]
+
+let mk_qvars (t:term) : term =
+  mk_app (`QVarS) [
+    (pack_ln Tv_Unknown, Q_Implicit);
+    (pack_ln Tv_Unknown, Q_Implicit);
+    (pack_ln Tv_Unknown, Q_Implicit);
+    (pack_ln Tv_Unknown, Q_Implicit);
+    (t, Q_Explicit)]
+
+let rec mk_qvarI (n:nat) : term =
+  if n = 0 then mk_qvar0
+  else mk_qvars (mk_qvarI (n-1))
+
+let mk_qlambda (body:term) : term =
+  mk_app (`QLambda) [
+    (pack_ln Tv_Unknown, Q_Implicit);
+    (pack_ln Tv_Unknown, Q_Implicit);
+    (pack_ln Tv_Unknown, Q_Implicit);
+    (pack_ln Tv_Unknown, Q_Implicit);
+    (body, Q_Explicit)]
+
+let mk_qapp (f arg : term) : term =
+  mk_app (`QApp) [
+    (pack_ln Tv_Unknown, Q_Implicit);
+    (pack_ln Tv_Unknown, Q_Implicit);
+    (pack_ln Tv_Unknown, Q_Implicit);
+    (pack_ln Tv_Unknown, Q_Implicit);
+    (pack_ln Tv_Unknown, Q_Implicit);
+    (f, Q_Explicit);
+    (arg, Q_Explicit)]
+
+noeq
+type fs_var =
+| FVar : fv -> fs_var
+| BVar : var -> fs_var
+
+type mapping =
+  fs_var -> option nat
+
+let empty_mapping : mapping = fun _ -> None
+
+let incr_option (x:option nat) : option nat =
+  match x with
+  | Some n -> Some (n+1)
+  | None -> None
+
+let extend_gmap_binder (gmap:mapping)
+  : mapping =
+  (fun x -> match x with
+      | BVar v -> if v = 0 then Some 0 else incr_option (gmap (BVar (v-1))) //Some v
+      | _ -> incr_option (gmap x))
+
+let extend_gmap (gmap:mapping) (b:string) : mapping =
+  (fun x -> match x with
+      | FVar v -> if fv_to_string v = b then Some 0 else (incr_option (gmap x))
+      | _ -> (incr_option (gmap x)))
+
+let rec exp_translation
+  g
+  (gmap:mapping)
+  (qfs:term)
+  : Tac term =
+  print ("      in exp translation: " ^ tag_of qfs);
+  match inspect_ln qfs with
+  // | Tv_FVar fv -> begin
+  //   let fnm = fv_to_string fv in
+  //   print ("    def: " ^ fnm ^ "\n");
+  //   let qdef' = norm_term_env g [delta_only [fnm]; zeta] qfs in
+  //   match inspect_ln qdef' with
+  //   | Tv_FVar fv' ->
+  //     if fnm = fv_to_string fv' then fail (fnm ^ " does not unfold!")
+  //     else exp_translation g gmap qdef'
+  //   | _ -> exp_translation g gmap qdef'
+  //   // print ("        looking for fvar: " ^ fv_to_string fv);
+  //   // match gmap (FVar fv) with
+  //   // | Some v -> mk_qvarI v
+  //   // | None -> fail (fv_to_string fv ^ " not defined")
+  // end
+
+  | Tv_BVar v -> begin
+    let i = (inspect_bv v).index in
+    match gmap (BVar i) with
+    | Some i' -> mk_qvarI i'
+    | None -> fail (print_nat i ^ " not defined")
+  end
+
+  | Tv_Abs bin body -> mk_qlambda (exp_translation g (extend_gmap_binder gmap) body)
+  | Tv_App hd (a, _) -> mk_qapp (exp_translation g gmap hd) (exp_translation g gmap a)
+
+  | Tv_Const C_Unit -> mk_qtt
+  | Tv_Const C_True -> mk_qtrue
+  | Tv_Const C_False -> mk_qfalse
+
+  | Tv_AscribedC t c _ _ -> begin
+    match inspect_comp c with
+    | C_Total _ -> exp_translation g gmap t
+    | _ -> fail ("not a total function type")
+  end
+
+  | _ -> fail ("not implemented: " ^ tag_of qfs)
+
+let rec def_translation g (gmap:mapping) (qdef:term) : Tac (string * term) =
+  print "  in def translation\n";
+  match inspect_ln qdef with
+  | Tv_FVar fv -> begin
+    let fnm = fv_to_string fv in
+    print ("    def: " ^ fnm ^ "\n");
+    let qdef' = norm_term_env g [delta_only [fnm]; zeta] qdef in
+    match inspect_ln qdef' with
+    | Tv_FVar fv' ->
+      if fnm = fv_to_string fv' then fail (fnm ^ " does not unfold!")
+      else def_translation g gmap qdef'
+    | _ -> (fnm, exp_translation g gmap qdef')
+  end
+  | _ -> fail ("not top-level definition")
+
+let meta_translation (nm:string) (qprog:term) (qtyp:term): dsl_tac_t = fun (g, expected_t) ->
   match expected_t with
   | Some t -> fail ("expected type " ^ tag_of t ^ " not supported")
   | None -> begin
-    let qderivation = mk_qtt in
-    let qtyp_derivation = mk_tyj (`QTyp.qUnit) qprog in
+    let qtyp_derivation = mk_tyj qtyp qprog in
+    let (_, qderivation) = def_translation g empty_mapping qprog in
+    match instantiate_implicits g qderivation (Some qtyp_derivation) true with
+    | (Some (_, qderivation', qtyp_derivation'), _) ->
+      let qderivation' = norm_term_env g [delta_only [
+ //        `%QTyp.fs_oval; `%QTyp.qUnit; `%QTyp.qBool; `%QTyp.qResexn; `%QTyp.op_Hat_Subtraction_Greater; `%QTyp.op_Hat_Star; `%QTyp.op_Hat_Plus; `%QTyp.get_rel; `%QTyp.get_Type; `%Mkdtuple2?._1;`%Mkdtuple2?._2;
+        `%QExp.helper_oval;
+	`%QTyp.fs_oval_lambda;`%QTyp.fs_oval_return;`%QTyp.fs_oval_var0;`%QTyp.fs_oval_varS;
+        `%QTyp.fs_oval_app]; zeta; iota; simplify] qderivation' in
 
-    ([], mk_unchecked_let g (cur_module ()) nm qderivation qtyp_derivation, [])
+      // type_dynamically g qtyp_derivation' qderivation';
+      ([], mk_unchecked_let g (cur_module ()) nm qderivation' qtyp_derivation', [])
+    | _ -> fail "could not instantiate implicits in derivation"
   end
 
-let src1 : unit = ()
-%splice_t[tgt1] (meta_translation "tgt1" (`src1))
+open QTyp
 
-let _ =
-  assert (tgt1 == Qtt)
+%splice_t[tgt1] (meta_translation "tgt1" (`Examples.ut_unit) (`qUnit))
+let _ = assert (tgt1 == test_ut_unit) by (trefl ())
+
+%splice_t[tgt2] (meta_translation "tgt2" (`Examples.ut_true) (`qBool))
+let _ = assert (tgt2 == test_ut_true) by (trefl ())
+
+%splice_t[tgt3] (meta_translation "tgt3" (`Examples.ut_false) (`qBool))
+let _ = assert (tgt3 == test_ut_false) by (trefl ())
+
+%splice_t[tgt4] (meta_translation "tgt4" (`Examples.constant) (`(qBool ^-> qBool)))
+let _ = assert (tgt4 == test_constant) by (trefl ())
+
+%splice_t[tgt5] (meta_translation "tgt5" (`Examples.identity) (`(qBool ^-> qBool)))
+let _ = assert (tgt5 == test_identity) by (trefl ())
+
+%splice_t[tgt6] (meta_translation "tgt6" (`Examples.thunked_id) (`(qBool ^-> qBool ^-> qBool)))
+let _ = assert (tgt6 == test_thunked_id) by (trefl ())
+
+%splice_t[tgt7] (meta_translation "tgt7" (`Examples.proj1) (`(qBool ^-> qBool ^-> qBool ^-> qBool)))
+let _ = assert (tgt7 == test_proj1) by (trefl ())
+%splice_t[tgt8] (meta_translation "tgt8" (`Examples.proj2) (`(qBool ^-> qBool ^-> qBool ^-> qBool)))
+let _ = assert (tgt8 == test_proj2) by (trefl ())
+%splice_t[tgt9] (meta_translation "tgt9" (`Examples.proj3) (`(qBool ^-> qBool ^-> qBool ^-> qBool)))
+let _ = assert (tgt9 == test_proj3) by (trefl ())
+
+%splice_t[tgt10] (meta_translation "tgt10" (`Examples.apply_arg) (`((qUnit ^-> qUnit) ^-> qUnit)))
+let _ = assert (tgt10 == test_apply_arg) by (trefl ())
+
+// TODO: why is this failing?
+%splice_t[tgt11] (meta_translation "tgt11" (`Examples.apply_arg2) (`((qBool ^-> qBool ^-> qBool) ^-> qBool)))
+let _ = assert (tgt11 == test_apply_arg2 ()) by (trefl ())
+
+%splice_t[tgt12] (meta_translation "tgt12" (`Examples.papply_arg2) (`((qBool ^-> qBool ^-> qBool) ^-> qBool ^-> qBool)))
+let _ = assert (tgt12 == test_papply_arg2 ()) by (trefl ())
